engine/evd.mli
@@ -680,6 +680,10 @@ val univ_entry : poly:bool -> evar_map -> UState.named_universes_entry
 
 val check_univ_decl : poly:bool -> evar_map -> UState.universe_decl -> UState.named_universes_entry
 
+(** An early check of compatibility of the universe declaration before
+    starting to build a declaration interactively *)
+val check_univ_decl_early : poly:bool -> evar_map -> UState.universe_decl -> Constr.t list -> unit
+
 val merge_universe_context : evar_map -> UState.t -> evar_map
 val set_universe_context : evar_map -> UState.t -> evar_map
 
